tests/lean/run/coinductive_predicates.lean
@@ -1,3 +1,27 @@
+open Lean.Order
+
+set_option trace.Elab.definition.partialFixpoint true
+
+@[partial_fixpoint_monotone] theorem monotone_exists
+    {α} [PartialOrder α] {β} (f : α → β → Prop)
+    (h : monotone f) :
+    monotone (fun x => Exists (f x)) :=
+  fun x y hxy ⟨w, hw⟩ => ⟨w, monotone_apply w f h x y hxy hw⟩
+
+@[partial_fixpoint_monotone] theorem monotone_and
+    {α} [PartialOrder α] (f₁ : α → Prop) (f₂ : α → Prop)
+    (h₁ : monotone f₁) (h₂ : monotone f₂) :
+    monotone (fun x => f₁ x ∧ f₂ x) :=
+  fun x y hxy ⟨hfx₁, hfx₂⟩ => ⟨h₁ x y hxy hfx₁, h₂ x y hxy hfx₂⟩
+
 def infinite_chain {α} (step : α → Option α) (x : α) : Prop :=
   ∃ y, step x = some y ∧ (infinite_chain step y)
   greatest_fixpoint
+
+theorem infinite_chain.coind {α} (P : α → Prop) (step : α → Option α)
+  (h : ∀ (x : α), P x → ∃ y, step x = some y ∧ P y) :
+  ∀ x, P x → infinite_chain step x := by
+    unfold infinite_chain
+    unfold gfp_monotone
+    apply (@gfp_coinduction (α → Prop) _)
+    exact h
